#! https://zhuanlan.zhihu.com/p/571063954
# 反演
$f_x=\sum\limits_{y=1}^nA_{x,y}g_y$

$g_x=\sum\limits_{y=1}^nB_{x,y}f_y$

把 $A,B$ 看成矩阵

满足上面式子的 $A,B$ 满足 $A*B=I$

所以已知 $f,A$ 可以求出 $A$ 的逆矩阵 $B$ 来求出 $g$
# 二项式反演
## 形式1
$A_{x,y}=\begin{cases}\dbinom yx&y\in[x,m]\\0&otherwise\end{cases}$

$B_{x,y}=\begin{cases}(-1)^{y-x}\dbinom yx&y\in[x,m]\\0&otherwise\end{cases}$
## 形式2
$A_{x,y}=\begin{cases}\dbinom xy&y\in[m,x]\\0&otherwise\end{cases}$

$B_{x,y}=\begin{cases}(-1)^{x-y}\dbinom xy&y\in[m,x]\\0&otherwise\end{cases}$